Two big subgoals left.

sepcomp/InliningproofEFF.v
@@ -61,38 +61,6 @@ Definition globalfunction_ptr_inject (j:meminj):=
               j b = Some(b,0) /\ isGlobalBlock SrcGe b = true. 
 
 (*The new match_states*)
-(*Inductive match_states (j:meminj): RTL_core -> mem -> RTL_core -> mem -> Prop :=
-| match_state:
-    forall f s k sp e m tm cs tf ns rs (*map ncont nexits ngoto nret rret*) sp'
-           (*(MWF: map_wf map)*)
-           (*(TS: tr_stmt tf.(fn_code) map s ns ncont nexits ngoto nret rret)*)
-           (*(TF: tr_fun tf map f ngoto nret rret)*)
-           (*(TK: tr_cont j tf.(fn_code) map k ncont nexits ngoto nret rret cs)*)
-           (*(ME: match_env j map e nil rs)*)
-           (*(MEXT: Mem.extends m tm)*)
-           (MINJ: Mem.inject j m tm)
-    (*(*NEW:*) (SP: sp_preserved j sp sp')*),
-      match_states j (RTL_State f s k sp e) m
-                   (RTL_State cs tf sp' ns rs) tm
-| match_callstate:
-    forall f args targs k m tm cs tf
-    (*(TF: transl_fundef f = OK tf)*)
-    (*(MS: match_stacks j k cs)*)
-    (*(LD: Val.lessdef_list args targs)*)
-    (*(AINJ: val_list_inject j args targs) *)
-    (*(MEXT: Mem.extends m tm)*)
-    (*(MINJ: Mem.inject j m tm)*),
-      match_states j (RTL_Callstate f args k) m
-                   (RTL_Callstate cs tf targs) tm
-| match_returnstate:
-    forall v tv k m tm cs
-    (*(MS: match_stacks j k cs)*)
-    (*(LD: Val.lessdef v tv)*)
-    (*(VINJ: val_inject j v tv)*)
-    (*(MEXT: Mem.extends m tm)*)
-    (*(MINJ: Mem.inject j m tm)*),
-      match_states j (RTL_Returnstate v k) m
-                   (RTL_Returnstate cs tv) tm.*)
 
 (*Tool kit for match states: *)
 
@@ -183,8 +151,8 @@ with match_stacks_inside (mu: SM_Injection) (m m': mem):
       match_stacks_inside (mu) m m' (Stackframe res f (Vptr sp Int.zero) pc rs :: stk)
                                  stk' f' ctx sp' rs'.
 
-Inductive match_states: RTL_core -> mem -> RTL_core -> mem -> Prop :=
-  | match_regular_states: forall (mu: SM_Injection) stk f sp pc rs m stk' f' sp' rs' m' ctx
+Inductive match_states:  SM_Injection -> RTL_core -> mem -> RTL_core -> mem -> Prop :=
+  | match_regular_states: forall mu stk f sp pc rs m stk' f' sp' rs' m' ctx
         (MS: match_stacks_inside mu m m' stk stk' f' ctx sp' rs')
         (FB: tr_funbody fenv f'.(fn_stacksize) ctx f f'.(fn_code))
         (AG: agree_regs (as_inj mu) ctx rs rs')
@@ -194,14 +162,14 @@ Inductive match_states: RTL_core -> mem -> RTL_core -> mem -> Prop :=
         (PRIV: range_private (as_inj mu) m m' sp' (ctx.(dstk) + ctx.(mstk)) f'.(fn_stacksize))
         (SSZ1: 0 <= f'.(fn_stacksize) < Int.max_unsigned)
         (SSZ2: forall ofs, Mem.perm m' sp' ofs Max Nonempty -> 0 <= ofs <= f'.(fn_stacksize)),
-      match_states (RTL_State stk f (Vptr sp Int.zero) pc rs) m
+      match_states mu (RTL_State stk f (Vptr sp Int.zero) pc rs) m
                    (RTL_State stk' f' (Vptr sp' Int.zero) (spc ctx pc) rs') m'
   | match_call_states: forall (mu: SM_Injection) stk fd args m stk' fd' args' m'
         (MS: match_stacks mu m m' stk stk' (Mem.nextblock m'))
         (FD: transf_fundef fenv fd = OK fd')
         (VINJ: val_list_inject  (as_inj mu) args args')
         (MINJ: Mem.inject (as_inj mu) m m'),
-      match_states (RTL_Callstate stk fd args) m
+      match_states mu (RTL_Callstate stk fd args) m
                    (RTL_Callstate stk' fd' args') m'
   | match_call_regular_states: forall (mu: SM_Injection) stk f vargs m stk' f' sp' rs' m' ctx ctx' pc' pc1' rargs
         (MS: match_stacks_inside mu m m' stk stk' f' ctx sp' rs')
@@ -215,13 +183,13 @@ Inductive match_states: RTL_core -> mem -> RTL_core -> mem -> Prop :=
         (PRIV: range_private  (as_inj mu) m m' sp' ctx.(dstk) f'.(fn_stacksize))
         (SSZ1: 0 <= f'.(fn_stacksize) < Int.max_unsigned)
         (SSZ2: forall ofs, Mem.perm m' sp' ofs Max Nonempty -> 0 <= ofs <= f'.(fn_stacksize)),
-      match_states (RTL_Callstate stk (Internal f) vargs) m
+      match_states mu (RTL_Callstate stk (Internal f) vargs) m
                    (RTL_State stk' f' (Vptr sp' Int.zero) pc' rs') m'
   | match_return_states: forall (mu: SM_Injection) stk v m stk' v' m'
         (MS: match_stacks mu m m' stk stk' (Mem.nextblock m'))
         (VINJ: val_inject (as_inj mu) v v')
         (MINJ: Mem.inject (as_inj mu) m m'),
-      match_states (RTL_Returnstate stk v) m
+      match_states mu (RTL_Returnstate stk v) m
                    (RTL_Returnstate stk' v') m'
   | match_return_regular_states: forall (mu: SM_Injection)stk v m stk' f' sp' rs' m' ctx pc' or rinfo
         (MS: match_stacks_inside mu m m' stk stk' f' ctx sp' rs')
@@ -233,18 +201,19 @@ Inductive match_states: RTL_core -> mem -> RTL_core -> mem -> Prop :=
         (PRIV: range_private (as_inj mu) m m' sp' ctx.(dstk) f'.(fn_stacksize))
         (SSZ1: 0 <= f'.(fn_stacksize) < Int.max_unsigned)
         (SSZ2: forall ofs, Mem.perm m' sp' ofs Max Nonempty -> 0 <= ofs <= f'.(fn_stacksize)),
-      match_states (RTL_Returnstate stk v) m
+      match_states mu (RTL_Returnstate stk v) m
                    (RTL_State stk' f' (Vptr sp' Int.zero) pc' rs') m'.
 
 
 Definition MATCH (d:RTL_core) mu c1 m1 c2 m2:Prop :=
-  match_states (*(restrict (as_inj mu) (vis mu))*) c1 m1 c2 m2 /\
+  match_states mu c1 m1 c2 m2 /\
   REACH_closed m1 (vis mu) /\
   meminj_preserves_globals SrcGe (as_inj mu) /\
-  globalfunction_ptr_inject (as_inj mu) /\
   (forall b, isGlobalBlock SrcGe b = true -> frgnBlocksSrc mu b = true) /\
-  sm_valid mu m1 m2 /\ SM_wd mu /\ Mem.inject (as_inj mu) m1 m2.
-
+  sm_valid mu m1 m2 /\
+  SM_wd mu /\
+  Mem.inject (as_inj mu) m1 m2 /\ 
+  globalfunction_ptr_inject (as_inj mu) .
 
 (** The simulation proof *)
 Theorem transl_program_correct:
@@ -298,38 +267,48 @@ Proof. intros.
   apply restrictI_Some; try eassumption.
   apply (Glob _ H1).
 Qed.
+
 Lemma MATCH_restrict: forall (d : RTL_core) (mu : SM_Injection) (c1 : RTL_core) 
                                  (m1 : mem) (c2 : RTL_core) (m2 : mem) (X : block -> bool) (MC: MATCH d mu c1 m1 c2 m2)(HX: forall b : block, vis mu b = true -> X b = true)(RC0:REACH_closed m1 X), MATCH d (restrict_sm mu X) c1 m1 c2 m2.
 intros.
 Proof. intros.
-  destruct MC as [MS [RC [PG [GFP [Glob [SMV [WD INJ]]]]]]].
+  destruct MC as [MC [RC [PG [GF [VAL [WDmu [INJ GFP]]]]]]].
 assert (WDR: SM_wd (restrict_sm mu X)).
    apply restrict_sm_WD; assumption.
+
 split.
-  (*rewrite vis_restrict_sm.*)
-  (*rewrite restrict_sm_all.*)
-  (*rewrite restrict_nest;*) intuition.
+
+Lemma match_states_restrict: forall mu m1 m2 c1 c2 X
+      (HX: forall b, vis mu b = true -> X b = true)
+      (RC: REACH_closed m1 X)
+      (MCS: match_states mu c1 m1 c2 m2 ),
+      match_states (restrict_sm mu X) c1 m1 c2 m2.
+admit.
+Qed.
+apply match_states_restrict; intuition.
+
 split. unfold vis.
   rewrite restrict_sm_locBlocksSrc, restrict_sm_frgnBlocksSrc.
   apply RC.
-split. clear -PG Glob HX.
+split. (*clear -PG HX.*)
   eapply restrict_sm_preserves_globals; try eassumption.
   unfold vis in HX. intuition.
-split. rewrite restrict_sm_all.
+split. 
+  rewrite restrict_sm_frgnBlocksSrc. apply GF.
+split.
+destruct VAL.
+(*This should be a lemma*)
+unfold sm_valid.
+    rewrite restrict_sm_DOM.
+    rewrite restrict_sm_RNG.
+    split; intros; intuition.
+split. assumption.
+split.
+ rewrite restrict_sm_all.
+eapply  inject_restrict; assumption.
+ rewrite restrict_sm_all.
   eapply restrict_preserves_globalfun_ptr; try eassumption.
   unfold vis in HX. intuition.
-split. 
-  rewrite restrict_sm_frgnBlocksSrc. apply Glob.
-split. 
-  destruct SMV.
-  split; intros.
-    rewrite restrict_sm_DOM in H1.
-    apply (H _ H1).
-  rewrite restrict_sm_RNG in H1.
-    apply (H0 _ H1).
-split. assumption.
-  rewrite restrict_sm_all.
-  eapply inject_restrict; eassumption.
 Qed.
 Hint Resolve MATCH_restrict: trans_correct.
 auto with trans_correct.
@@ -361,11 +340,67 @@ Qed.
 Hint Resolve MATCH_PG: trans_correct.
 eauto with trans_correct.
 
-admit.
+Lemma MATCH_initial_core: forall (v1 v2 : val) (sig : signature) entrypoints
+  (entry_points_ok : forall (v1 v2 : val) (sig : signature),
+                    In (v1, v2, sig) entrypoints ->
+                    exists (b : block) (f1 f2 : fundef),
+                      v1 = Vptr b Int.zero /\
+                      v2 = Vptr b Int.zero /\
+                      Genv.find_funct_ptr SrcGe b = Some f1 /\
+                      Genv.find_funct_ptr TrgGe b = Some f2)
+   (EP: In (v1, v2, sig) entrypoints)
+   (vals1 : list val) (c1 : RTL_core) (m1 : mem) 
+     (j : meminj) (vals2 : list val) (m2 : mem) (DomS DomT : block -> bool)
+   (SM_Ini:initial_core rtl_eff_sem SrcGe v1 vals1 = Some c1)
+   (Inj: Mem.inject j m1 m2)
+   (VInj: Forall2 (val_inject j) vals1 vals2)
+   (PG: meminj_preserves_globals SrcGe j)
+   (J: forall (b1 b2 : block) (d : Z),
+    j b1 = Some (b2, d) -> DomS b1 = true /\ DomT b2 = true)
+   (RCH: forall b : block,
+    REACH m2 (fun b' : block => isGlobalBlock TrgGe b' || getBlocks vals2 b')
+      b = true -> DomT b = true)
+   (HDomS: (forall b : block, DomS b = true -> Mem.valid_block m1 b))
+   (HDomT: (forall b : block, DomT b = true -> Mem.valid_block m2 b)),
+   exists c2 : RTL_core,
+     initial_core rtl_eff_sem TrgGe v2 vals2 = Some c2 /\
+     MATCH c1
+       (initial_SM DomS DomT
+          (REACH m1
+             (fun b : block => isGlobalBlock SrcGe b || getBlocks vals1 b))
+          (REACH m2
+             (fun b : block => isGlobalBlock TrgGe b || getBlocks vals2 b)) j)
+       c1 m1 c2 m2.
+ Proof.
+  intros.
+  inversion SM_Ini.
+  unfold  RTL_initial_core in H0. unfold SrcGe in *. unfold TrgGe in *.
+  destruct v1; inv H0.
+  remember (Int.eq_dec i Int.zero) as z; destruct z; inv H1. clear Heqz.
+  remember (Genv.find_funct_ptr (Genv.globalenv SrcProg) b) as zz; destruct zz; inv H0. 
+    apply eq_sym in Heqzz.
+  exploit function_ptr_translated; eauto. intros [tf [FIND TR]].
+  exists (RTL_Callstate nil tf vals2).
+  split. 
+  simpl. 
+  destruct (entry_points_ok _ _ _ EP) as [b0 [f1 [f2 [A [B [C D]]]]]].
+  subst. inv A. rewrite C in Heqzz. inv Heqzz. 
+  unfold SrcGe, TrgGe in *.
+  rewrite D in FIND. inv FIND.
+  unfold RTL_initial_core. 
+  case_eq (Int.eq_dec Int.zero Int.zero). intros ? e.
+  solve[rewrite D; auto].
+  intros CONTRA.
+  solve[elimtype False; auto].
+  (*destruct InitMem as [m0 [INIT_MEM [A B]]].*)
+  admit.
+Qed.
+Hint Resolve MATCH_initial_core: trans_correct.
+eauto with trans_correct.
 
 Lemma Match_Halted: forall (cd : RTL_core) (mu : SM_Injection) (c1 : RTL_core) 
      (m1 : mem) (c2 : RTL_core) (m2 : mem) (v1 : val)(MC:
-   MATCH cd mu c1 m1 c2 m2)(HL:
+   MATCH cd mu c1 m1 c2 m2)(HALT:
    halted rtl_eff_sem c1 = Some v1),
    exists v2 : val,
      Mem.inject (as_inj mu) m1 m2 /\
@@ -373,262 +408,390 @@ Lemma Match_Halted: forall (cd : RTL_core) (mu : SM_Injection) (c1 : RTL_core)
      halted rtl_eff_sem c2 = Some v2.
 Proof.
 intros.
-inv MC.
-repeat  match goal with
-      | H: _ /\ _ |- _ => inv H
-  end.
-Print val_inject.
-destruct H.
-(*match_regular_states*)
-eexists v1.
-split; try assumption.
-split. 
-Focus 2.
+unfold MATCH in MC; destruct MC as [H0 H1].
+inv H0; simpl in *; inv HALT. 
+Print match_states.
+inv MS. 
+exists v'; split; try assumption; split; try reflexivity; inv H0. admit.
+inv H0.
+inv MS0; [rewrite RET in RET0; inv RET0 | inv H0].
+inv MS.
+rewrite RET in RET0; inv RET0.
+inv H0.
+Qed.
+Hint Resolve Match_Halted: trans_correct.
+eauto with trans_correct.
 
-
-destruct v1; try constructor.
-Print val_inject.
-eapply val_inject_ptr.
-
-(*match_call_states*)
-(*match_call_regular_states*)
-(*match_return_states*)
-(*match_return_regular_states*)
-
-
-eexists.
-split. apply H7.
-induction H.
-
-
-
-
-
-
-
-
-
-
-Lemma MATCH_safely_halted: forall mu c1 m1 c2 m2 v1
-     (SMC: match_states c1 m1 c2 m2)
-     (HALT: halted rtl_eff_sem c1 = Some v1),
-exists v2, halted rtl_eff_sem c2 = Some v2 /\ 
-           val_inject (restrict (as_inj mu) (vis mu)) v1 v2.
-Proof.
+Lemma at_external_lemma: forall (mu : SM_Injection) (c1 : RTL_core) (m1 : mem) 
+                                (c2 : RTL_core) (m2 : mem) (e : external_function) 
+                                (vals1 : list val) (ef_sig : signature)(MC: MATCH c1 mu c1 m1 c2 m2) (ATE: at_external rtl_eff_sem c1 = Some (e, ef_sig, vals1)),
+                           Mem.inject (as_inj mu) m1 m2 /\ 
+                           (exists vals2 : list val, Forall2 (val_inject (restrict (as_inj mu) (vis mu))) vals1 vals2 /\ at_external rtl_eff_sem c2 = Some (e, ef_sig, vals2)).
   intros.
-  inv SMC; simpl in *; inv HALT.
-  destruct stk; inv H0.
-  destruct stk'.
-  exists v'; split; try reflexivity.
+  split. inv MC; apply H0.
+  inv MC; simpl in *. inv H; inv ATE.
+  destruct fd; inv H1.
+  exists args'.
+  split. apply val_list_inject_forall_inject. admit.
+  inv FD; trivial.
+Qed.
+Hint Resolve at_external_lemma: trans_correct.
+eauto with trans_correct.
 
-  (*eapply restrict_val_inject.*) eapply VINJ.
-exists nil.
-  inv MK. split; trivial.
-(*  eapply val_inject_incr; try eassumption.
-    apply restrict_incr.*)
-Qed.*)
-
-
-
-
-Lemma MATCH_initial_core: forall v1 v2 sig entrypoints
-      (EP: In (v1, v2, sig) entrypoints)
-      (entry_points_ok : forall (v1 v2 : val) (sig : signature),
-                  In (v1, v2, sig) entrypoints ->
-                  exists b f1 f2,
-                    v1 = Vptr b Int.zero /\
-                    v2 = Vptr b Int.zero /\
-                    Genv.find_funct_ptr SrcGe b = Some f1 /\
-                    Genv.find_funct_ptr TrgGe b = Some f2)
-      vals1 c1 m1 j vals2 m2 (DomS DomT : block -> bool)
-      (Ini: initial_core rtl_eff_sem SrcGe v1 vals1 = Some c1)
-      (Inj: Mem.inject j m1 m2)
-      (VInj: Forall2 (val_inject j) vals1 vals2)
-      (PG:meminj_preserves_globals SrcGe j)
-      (R : list_norepet (map fst (prog_defs SrcProg)))
-      (J: forall b1 b2 delta, j b1 = Some (b2, delta) -> 
-            (DomS b1 = true /\ DomT b2 = true))
-      (RCH: forall b, REACH m2 
-          (fun b' : block => isGlobalBlock TrgGe b' || getBlocks vals2 b') b = true ->
-          DomT b = true)
-      (InitMem : exists m0 : mem, Genv.init_mem SrcProg = Some m0 
-               /\ Ple (Mem.nextblock m0) (Mem.nextblock m1) 
-               /\ Ple (Mem.nextblock m0) (Mem.nextblock m2))   
-      (GDE: genvs_domain_eq SrcGe TrgGe)
-      (HDomS: forall b : block, DomS b = true -> Mem.valid_block m1 b)
-      (HDomT: forall b : block, DomT b = true -> Mem.valid_block m2 b),
-exists c2,
-  initial_core rtl_eff_sem TrgGe v2 vals2 = Some c2 /\
-  MATCH c1
-    (initial_SM DomS DomT
-       (REACH m1 (fun b : block => isGlobalBlock SrcGe b || getBlocks vals1 b))
-       (REACH m2 (fun b : block => isGlobalBlock TrgGe b || getBlocks vals2 b))
-       j) c1 m1 c2 m2.
-  intros.
-  inversion Ini.
-  unfold RTL_initial_core in H0. unfold ge in *. unfold TrgGe in *.
-  destruct v1; inv H0.
-  remember (Int.eq_dec i Int.zero) as z; destruct z; inv H1. clear Heqz.
-  remember (Genv.find_funct_ptr (Genv.globalenv SrcProg) b) as zz. destruct zz. 
-  unfold SrcGe in H0. inv H0. 
-    apply eq_sym in Heqzz.
-  rewrite Heqzz in H1.
-  exploit function_ptr_translated; eauto. intros [tf [FP TF]].
-  exists (RTL_Callstate nil tf vals2).
-  split.
-    destruct (entry_points_ok _ _ _ EP) as [b0 [f1 [f2 [A [B [C D]]]]]].
-    subst. inv A. unfold SrcGe in *; rewrite C in Heqzz. inv Heqzz. 
-    unfold TrgGe in FP. rewrite D in FP. inv FP.
-    unfold rtl_eff_sem. simpl.
-    case_eq (Int.eq_dec Int.zero Int.zero). intros ? e.
-    solve[rewrite D; auto].
-
-    intros CONTRA; contradiction CONTRA; reflexivity.
-    inv H1.
-
-(*  assert (exists targs tres, type_of_fundef f = Tfunction targs tres).
-         destruct f; simpl. eexists; eexists. reflexivity.
-         eexists; eexists. reflexivity.
-  destruct H as [targs [tres Tfun]].*)
-  destruct (core_initial_wd SrcGe TrgGe _ _ _ _ _ _ _  Inj
-     VInj J RCH PG GDE HDomS HDomT _ (eq_refl _))
-    as [AA [BB [CC [DD [EE [FF GG]]]]]].
-  split.
-    eapply match_call_states; try eassumption.
-      econstructor.
-      Print match_globalenvs.
-      Print initial_SM_as_inj.
-      rewrite initial_SM_as_inj.
-        unfold vis, initial_SM; simpl.
-        apply forall_inject_val_list_inject.
-        eapply restrict_forall_vals_inject; try eassumption.
-          intros. apply REACH_nil. rewrite H; intuition.
-    rewrite initial_SM_as_inj.
-      unfold vis, initial_SM; simpl.
-      eapply inject_restrict; eassumption.
-  intuition.
-    rewrite match_genv_meminj_preserves_extern_iff_all.
+Lemma Match_AfterExternal: 
+forall (mu : SM_Injection) (st1 : RTL_core) (st2 : RTL_core) (m1 : mem) (e : external_function) (vals1 : list val) (m2 : mem) (ef_sig : signature) (vals2 : list val) (e' : external_function) (ef_sig' : signature) 
+       (MemInjMu : Mem.inject (as_inj mu) m1 m2)
+       (MatchMu : MATCH st1 mu st1 m1 st2 m2)
+       (AtExtSrc : at_external rtl_eff_sem st1 = Some (e, ef_sig, vals1))
+       (AtExtTgt : at_external rtl_eff_sem st2 = Some (e', ef_sig', vals2))
+       (ValInjMu : Forall2 (val_inject (restrict (as_inj mu) (vis mu))) vals1 vals2)
+       (pubSrc' : block -> bool)
+       (pubSrcHyp : pubSrc' =
+              (fun b : block =>
+               locBlocksSrc mu b && REACH m1 (exportedSrc mu vals1) b))
+       (pubTgt' : block -> bool)
+       (pubTgtHyp : pubTgt' =
+              (fun b : block =>
+               locBlocksTgt mu b && REACH m2 (exportedTgt mu vals2) b))
+       (nu : SM_Injection)
+       (NuHyp : nu = replace_locals mu pubSrc' pubTgt')
+       (nu' : SM_Injection)
+       (ret1 : val)
+       (m1' : mem)
+       (ret2 : val)
+       (m2' : mem)
+       (INC : extern_incr nu nu')
+       (SEP : sm_inject_separated nu nu' m1 m2)
+       (WDnu' : SM_wd nu')
+       (SMvalNu' : sm_valid nu' m1' m2')
+       (MemInjNu' : Mem.inject (as_inj nu') m1' m2')
+       (RValInjNu' : val_inject (as_inj nu') ret1 ret2)
+       (FwdSrc : mem_forward m1 m1')
+       (FwdTgt : mem_forward m2 m2')
+       (frgnSrc' : block -> bool)
+       (frgnSrcHyp : frgnSrc' =
+               (fun b : block =>
+                DomSrc nu' b &&
+                (negb (locBlocksSrc nu' b) &&
+                 REACH m1' (exportedSrc nu' (ret1 :: nil)) b)))
+       (frgnTgt' : block -> bool)
+       (frgnTgtHyp : frgnTgt' =
+               (fun b : block =>
+                DomTgt nu' b &&
+                (negb (locBlocksTgt nu' b) &&
+                 REACH m2' (exportedTgt nu' (ret2 :: nil)) b)))
+       (mu' : SM_Injection)
+       (Mu'Hyp : mu' = replace_externs nu' frgnSrc' frgnTgt')
+       (UnchPrivSrc : Mem.unchanged_on
+                  (fun (b : block) (_ : Z) =>
+                   locBlocksSrc nu b = true /\ pubBlocksSrc nu b = false) m1 m1')
+       (UnchLOOR : Mem.unchanged_on (local_out_of_reach nu m1) m2 m2'),
+exists (st1' st2' : RTL_core),
+  after_external rtl_eff_sem (Some ret1) st1 = Some st1' /\
+  after_external rtl_eff_sem (Some ret2) st2 = Some st2' /\
+  MATCH st1' mu' st1' m1' st2' m2'.
+Proof. intros. 
+ destruct MatchMu as [MC [RC [PG [GF [VAL [WDmu [INJ GFP]]]]]]].
+ inv MC; simpl in *; inv AtExtSrc.
+  destruct fd; inv H0.
+  destruct fd'; inv AtExtTgt.
+  exists (RTL_Returnstate stk ret1). eexists.
+    split. reflexivity.
+    split. reflexivity.
+  simpl in *.
+inv FD.
+assert (INCvisNu': inject_incr
+  (restrict (as_inj nu')
+     (vis
+        (replace_externs nu'
+           (fun b : Values.block =>
+            DomSrc nu' b &&
+            (negb (locBlocksSrc nu' b) &&
+             REACH m1' (exportedSrc nu' (ret1 :: nil)) b))
+           (fun b : Values.block =>
+            DomTgt nu' b &&
+            (negb (locBlocksTgt nu' b) &&
+             REACH m2' (exportedTgt nu' (ret2 :: nil)) b))))) (as_inj nu')).
+      unfold vis. rewrite replace_externs_frgnBlocksSrc, replace_externs_locBlocksSrc.
+      apply restrict_incr. 
+assert (RC': REACH_closed m1' (mapped (as_inj nu'))).
+        eapply inject_REACH_closed; eassumption.
+assert (PHnu': meminj_preserves_globals (Genv.globalenv SrcProg) (as_inj nu')).
+    subst. clear - INC SEP PG GF WDmu WDnu'.
+    apply meminj_preserves_genv2blocks in PG.
+    destruct PG as [PGa [PGb PGc]].
+    apply meminj_preserves_genv2blocks.
+    split; intros.
+      specialize (PGa _ H).
+      apply joinI; left. apply INC.
+      rewrite replace_locals_extern.
+      apply foreign_in_extern.
+     assert (GG: isGlobalBlock SrcGe b = true).
+          unfold isGlobalBlock, SrcGe. apply genv2blocksBool_char1 in H.
+          rewrite H. trivial.
+      Check frgnSrc.
+      destruct (frgnSrc _ WDmu _ (GF _ GG)) as [bb2 [dd [FF FT2]]].
+      rewrite (foreign_in_all _ _ _ _ FF) in PGa. inv PGa.
       assumption.
-      apply BB.
-      apply EE.
-    (*as in selectionprffEFF*)
-    rewrite initial_SM_as_inj.
-      red; intros. specialize (Genv.find_funct_ptr_not_fresh prog). intros.
-         destruct InitMem as [m0 [INIT_MEM [? ?]]].
-         specialize (H0 _ _ _ INIT_MEM H). 
-         destruct (valid_init_is_global _ R _ INIT_MEM _ H0) as [id Hid]. 
-           destruct PG as [PGa [PGb PGc]]. split. eapply PGa; eassumption.
-         unfold isGlobalBlock. 
-          apply orb_true_iff. left. apply genv2blocksBool_char1.
-            simpl. exists id; eassumption.
-    rewrite initial_SM_as_inj; assumption.
+    split; intros. specialize (PGb _ H).
+      apply joinI; left. apply INC.
+      rewrite replace_locals_extern. 
+      assert (GG: isGlobalBlock SrcGe b = true). (*4 goals*)
+          unfold isGlobalBlock, SrcGe. apply genv2blocksBool_char2 in H.
+          rewrite H. intuition. (*3 goals*)
+      destruct (frgnSrc _ WDmu _ (GF _ GG)) as [bb2 [dd [FF FT2]]].
+      rewrite (foreign_in_all _ _ _ _ FF) in PGb. inv PGb.
+      apply foreign_in_extern; eassumption. (*2 goals*)
+    eapply (PGc _ _ delta H). specialize (PGb _ H). clear PGa PGc.
+      remember (as_inj mu b1) as d.
+      destruct d; apply eq_sym in Heqd. (*3 goals*)
+        destruct p. 
+        apply extern_incr_as_inj in INC; trivial. (*3 goals*)
+        rewrite replace_locals_as_inj in INC.
+        rewrite (INC _ _ _ Heqd) in H0. trivial. (*3 goals*)
+      destruct SEP as [SEPa _].
+        rewrite replace_locals_as_inj, replace_locals_DomSrc, replace_locals_DomTgt in SEPa. 
+        destruct (SEPa _ _ _ Heqd H0).
+        destruct (as_inj_DomRng _ _ _ _ PGb WDmu).
+        congruence. (*1 goal*)
+assert (RR1: REACH_closed m1'
+  (fun b : Values.block =>
+   locBlocksSrc nu' b
+   || DomSrc nu' b &&
+      (negb (locBlocksSrc nu' b) &&
+       REACH m1' (exportedSrc nu' (ret1 :: nil)) b))).
+  intros b Hb. rewrite REACHAX in Hb. destruct Hb as [L HL].
+  generalize dependent b.
+  induction L; simpl; intros; inv HL.
+     assumption.
+  specialize (IHL _ H1); clear H1.
+  apply orb_true_iff in IHL.
+  remember (locBlocksSrc nu' b') as l.
+  destruct l; apply eq_sym in Heql.
+  (*case locBlocksSrc nu' b' = true*)
+    clear IHL.
+    remember (pubBlocksSrc nu' b') as p.
+    destruct p; apply eq_sym in Heqp.
+      assert (Rb': REACH m1' (mapped (as_inj nu')) b' = true).
+        apply REACH_nil. 
+        destruct (pubSrc _ WDnu' _ Heqp) as [bb2 [dd1 [PUB PT]]].
+        eapply mappedI_true.
+         apply (pub_in_all _ WDnu' _ _ _ PUB).
+      assert (Rb:  REACH m1' (mapped (as_inj nu')) b = true).
+        eapply REACH_cons; try eassumption.
+      specialize (RC' _ Rb).
+      destruct (mappedD_true _ _ RC') as [[b2 d1] AI'].
+      remember (locBlocksSrc nu' b) as d.
+      destruct d; simpl; trivial.
+      apply andb_true_iff. 
+      split. eapply as_inj_DomRng; try eassumption.
+      eapply REACH_cons; try eassumption.
+        apply REACH_nil. unfold exportedSrc.
+        rewrite (pubSrc_shared _ WDnu' _ Heqp). intuition.
+      destruct (UnchPrivSrc) as [UP UV]; clear UnchLOOR.
+        specialize (UP b' z Cur Readable). 
+        specialize (UV b' z). 
+        destruct INC as [_ [_ [_ [_ [LCnu' [_ [PBnu' [_ [FRGnu' _]]]]]]]]].
+        rewrite <- LCnu'. rewrite replace_locals_locBlocksSrc.  
+        rewrite <- LCnu' in Heql. rewrite replace_locals_locBlocksSrc in *.
+        rewrite <- PBnu' in Heqp. rewrite replace_locals_pubBlocksSrc in *.
+        clear INCvisNu'. 
+        rewrite Heql in *. simpl in *. intuition.
+        assert (VB: Mem.valid_block m1 b').
+          eapply VAL. unfold DOM, DomSrc. rewrite Heql. intuition.
+        apply (H VB) in H2.
+        rewrite (H0 H2) in H4. clear H H0.
+        remember (locBlocksSrc mu b) as q.
+        destruct q; simpl; trivial; apply eq_sym in Heqq.
+        assert (Rb : REACH m1 (vis mu) b = true).
+           eapply REACH_cons; try eassumption.
+           apply REACH_nil. unfold vis. rewrite Heql; trivial.
+        specialize (RC _ Rb). unfold vis in RC.
+           rewrite Heqq in RC; simpl in *.
+        rewrite replace_locals_frgnBlocksSrc in FRGnu'.
+        rewrite FRGnu' in RC.
+        apply andb_true_iff.  
+        split. unfold DomSrc. rewrite (frgnBlocksSrc_extBlocksSrc _ WDnu' _ RC). intuition.
+        apply REACH_nil. unfold exportedSrc.
+          rewrite (frgnSrc_shared _ WDnu' _ RC). intuition.
+  (*case DomSrc nu' b' &&
+    (negb (locBlocksSrc nu' b') &&
+     REACH m1' (exportedSrc nu' (ret1 :: nil)) b') = true*)
+    destruct IHL. inv H.
+    apply andb_true_iff in H. simpl in H. 
+    destruct H as[DomNu' Rb']. 
+    clear INC SEP INCvisNu' UnchLOOR UnchPrivSrc.
+    remember (locBlocksSrc nu' b) as d.
+    destruct d; simpl; trivial. apply eq_sym in Heqd.
+    apply andb_true_iff.
+    split. assert (RET: Forall2 (val_inject (as_inj nu')) (ret1::nil) (ret2::nil)).
+              constructor. assumption. constructor.
+           destruct (REACH_as_inj _ WDnu' _ _ _ _ MemInjNu' RET
+               _ Rb' (fun b => true)) as [b2 [d1 [AI' _]]]; trivial.
+           assert (REACH m1' (mapped (as_inj nu')) b = true).
+             eapply REACH_cons; try eassumption.
+             apply REACH_nil. eapply mappedI_true; eassumption.
+           specialize (RC' _ H). 
+           destruct (mappedD_true _ _ RC') as [[? ?] ?].
+           eapply as_inj_DomRng; eassumption.
+    eapply REACH_cons; try eassumption.
+(*assert (RRR: REACH_closed m1' (exportedSrc nu' (ret1 :: nil))).
+    intros b Hb. apply REACHAX in Hb.
+       destruct Hb as [L HL].
+       generalize dependent b.
+       induction L ; simpl; intros; inv HL; trivial.
+       specialize (IHL _ H1); clear H1.
+       unfold exportedSrc.
+       eapply REACH_cons; eassumption.*)
 
+assert (RRC: REACH_closed m1' (fun b : Values.block =>
+                         mapped (as_inj nu') b &&
+                           (locBlocksSrc nu' b
+                            || DomSrc nu' b &&
+                               (negb (locBlocksSrc nu' b) &&
+                           REACH m1' (exportedSrc nu' (ret1 :: nil)) b)))).
+  eapply REACH_closed_intersection; eassumption.
+assert (GFnu': forall b, isGlobalBlock (Genv.globalenv SrcProg) b = true ->
+               DomSrc nu' b &&
+               (negb (locBlocksSrc nu' b) && REACH m1' (exportedSrc nu' (ret1 :: nil)) b) = true).
+     intros. specialize (GF _ H).
+       assert (FSRC:= extern_incr_frgnBlocksSrc _ _ INC).
+          rewrite replace_locals_frgnBlocksSrc in FSRC.
+       rewrite FSRC in GF.
+       rewrite (frgnBlocksSrc_locBlocksSrc _ WDnu' _ GF). 
+       apply andb_true_iff; simpl.
+        split.
+          unfold DomSrc. rewrite (frgnBlocksSrc_extBlocksSrc _ WDnu' _ GF). intuition.
+          apply REACH_nil. unfold exportedSrc.
+          rewrite (frgnSrc_shared _ WDnu' _ GF). intuition.
+split.
+  unfold vis in *.
+  rewrite replace_externs_frgnBlocksSrc, replace_externs_locBlocksSrc in *.
+  econstructor; try eassumption.
 
-
-
-
-
-
-
-
-
-
-
-
-
-
-
-
-
-(*Proof 0.2*)
-intros.
-  inversion Ini.
-  unfold  RTL_initial_core in H0. unfold SrcGe in *. unfold TrgGe in *.
-  destruct v1; inv H0.
-  remember (Int.eq_dec i Int.zero) as z; destruct z; inv H1. clear Heqz.
-  remember (Genv.find_funct_ptr (Genv.globalenv SrcProg) b) as zz; destruct zz; inv H0. 
-    apply eq_sym in Heqzz.
-  exploit function_ptr_translated; eauto. intros [tf [FIND TR]].
-  eexists (RTL_Callstate _ _ _).
-  split.
-  simpl. 
-  destruct (entry_points_ok _ _ _ EP) as [b0 [f1 [f2 [A [B [C D]]]]]].
-  subst. inv A. rewrite C in Heqzz. inv Heqzz. unfold TrgGe in *; rewrite D in FIND. inv FIND.
-  unfold RTL_initial_core. 
-  case_eq (Int.eq_dec Int.zero Int.zero). intros ? e.
-  solve[rewrite D; auto].
-  intros CONTRA.
-  solve[elimtype False; auto].
-  destruct InitMem as [m0 [INIT_MEM [A B]]].
-  split.
-  eapply match_call_states; try eassumption.
-  (*eapply RTL_Callstate (*with (cenv:=PTree.empty _)(cs := @nil frame)*); try eassumption.*)
-    eapply match_stacks_nil.
 (*
-        (MS: match_stacks F m m' stk stk' (Mem.nextblock m'))
-        (FD: transf_fundef fenv fd = OK fd')
-        (VINJ: val_list_inject F args args')
-        (MINJ: Mem.inject F m m'),
-*)
+Lemma structured_match_callstack_incr_bound:
+  forall f m tm cs bound tbound bound' tbound',
+  match_stacks f m tm cs bound (*tbound*) ->
+  Ple bound bound' -> Ple tbound tbound' ->
+  match_stacks f m tm cs bound' tbound'.
+Proof.
+  intros. inv H.
+  econstructor; eauto. xomega. xomega. 
+  constructor; auto. xomega. xomega.
 
-    (*assert (Genv.init_mem TrgProg = Some m0).*)
-    unfold match_globalenvs.
-      unfold transl_program in TRANSL.
-      solve[eapply Genv.init_mem_transf_partial in TRANSL; eauto].
-    (*rewrite initial_SM_as_inj. unfold vis. unfold initial_SM; simpl.
-      eapply inject_mapped; try eassumption.
-       eapply restrict_mapped_closed.
-         eapply inject_REACH_closed; eassumption.
-         apply REACH_is_closed.
-       apply restrict_incr.*)
-    (*rewrite initial_SM_as_inj. *)
-      apply st_mcs_nil with (Mem.nextblock m0).
-    eapply (match_globalenvs_init' _ R _ _ INIT_MEM).
-      (*rewrite restrict_sm_all.*) rewrite initial_SM_as_inj.
-      eapply restrict_preserves_globals; try eassumption.
-      unfold vis, initial_SM; simpl; intros.
-      apply REACH_nil. rewrite H0; trivial.
-    apply A. apply B.
-    econstructor. simpl. trivial.
-    (*rewrite restrict_sm_all.*) rewrite initial_SM_as_inj.
-      unfold vis, initial_SM; simpl.
-      apply forall_inject_val_list_inject.
-      eapply restrict_forall_vals_inject; try eassumption.
-        intros. apply REACH_nil. rewrite H; intuition.
-(*
-    eapply restrict_preserves_globals; try eassumption.
-      rewrite initial_SM_as_inj. assumption.
-      intros. unfold vis, initial_SM; simpl. 
-      apply REACH_nil. rewrite H; trivial.*)
-destruct (core_initial_wd ge tge _ _ _ _ _ _ _  Inj
-    VInj J RCH PG GDE HDomS HDomT _ (eq_refl _))
-   as [AA [BB [CC [DD [EE [FF GG]]]]]].
-intuition. rewrite initial_SM_as_inj. assumption.
-rewrite initial_SM_as_inj. assumption.
-(*protected: red. simpl. intros. discriminate.*)
+
+
+    eapply structured_match_callstack_incr_bound.
+Lemma structured_match_callstack_ext: forall mu m1 m2 cs bound 
+  tbound
+  (MCS : match_stacks mu m1 m2 cs bound tbound)
+  m1' (FwdSrc : mem_forward m1 m1')
+  nu vals1 vals2
+  (Hnu: nu = replace_locals mu
+                      (fun b0 : Values.block =>
+                       locBlocksSrc mu b0 &&
+                       REACH m1 (exportedSrc mu vals1) b0)
+                      (fun b0 : Values.block =>
+                       locBlocksTgt mu b0 &&
+                       REACH m2 (exportedTgt mu vals2) b0))
+  (SMvalMu : sm_valid mu m1 m2)
+  (PG : meminj_preserves_globals (Genv.globalenv SrcProg) (as_inj mu))
+  nu' (INC : extern_incr nu nu')
+  (SEP : sm_inject_separated nu nu' m1 m2)
+  (UNMAPPED : Mem.unchanged_on
+                (fun (b : Values.block) (_ : Z) =>
+                 locBlocksSrc nu b = true /\ pubBlocksSrc nu b = false) m1
+                m1')
+   m2' (FwdTgt : mem_forward m2 m2') (OUTOFREACH : Mem.unchanged_on (local_out_of_reach nu m1) m2 m2')
+  ret1 ret2 (WDnu' : SM_wd nu') (WDmu : SM_wd mu) (WDnu : SM_wd nu)
+  (BND: Ple bound (Mem.nextblock m1))
+  (TBND:Ple tbound (Mem.nextblock m2)),
+match_stacks
+  (replace_externs nu'
+        (fun b : Values.block =>
+         DomSrc nu' b &&
+         (negb (locBlocksSrc nu' b) && REACH m1' (exportedSrc nu' (ret1 :: nil)) b))
+        (fun b : Values.block =>
+         DomTgt nu' b &&
+         (negb (locBlocksTgt nu' b) && REACH m2' (exportedTgt nu' (ret2 :: nil)) b)))
+   m1' m2' cs bound tbound.
+Proof.
+
+
+
+      eapply structured_match_callstack_ext with
+       (mu:=mu)(nu':=nu'); try reflexivity; try eassumption.
+       eapply eff_after_check1 with (mu:=mu); try eassumption; try reflexivity.
+         eapply forall_vals_inject_restrictD; eassumption.
+       apply (forward_nextblock _ _ FwdSrc).
+       apply (forward_nextblock _ _ FwdTgt).*)
+admit.
+Check replace_externs_as_inj.
+    rewrite replace_externs_as_inj. assumption.
+    (*Check restrict_val_inject.
+    eapply restrict_val_inject; try eassumption.
+    Print restrict_val_inject.
+      (*eapply restrict_val_inject; try eassumption.*)
+    intros.
+        destruct (getBlocks_inject (as_inj nu') (ret1::nil) (ret2::nil))
+           with (b:=b) as [bb [dd [JJ' GBbb]]]; try eassumption.
+          constructor. assumption. constructor.
+         unfold vis. rewrite replace_externs_frgnBlocksSrc, replace_externs_locBlocksSrc.
+        remember (locBlocksSrc nu' b) as d.
+        destruct d; simpl; trivial. apply andb_true_iff.
+        split. eapply as_inj_DomRng; eassumption.
+        apply REACH_nil. unfold exportedSrc.
+           rewrite H. trivial.*)
+admit.
+unfold vis.
+rewrite replace_externs_locBlocksSrc, replace_externs_frgnBlocksSrc,
+        replace_externs_as_inj.
+destruct (eff_after_check2 _ _ _ _ _ MemInjNu' RValInjNu' 
+      _ (eq_refl _) _ (eq_refl _) _ (eq_refl _) WDnu' SMvalNu').
+intuition.
+unfold globalfunction_ptr_inject.
+admit.
 Qed.
 
+Hint Resolve Match_AfterExternal: trans_correct.
+eauto with trans_correct.
+
+unfold   well_founded.
+Print Acc.
 
 
 
 
-Lemma MATCH_safely_halted: forall mu c1 m1 c2 m2 v1
-     (SMC: match_states c1 m1 c2 m2)
-     (HALT: halted rtl_eff_sem c1 = Some v1),
-exists v2, halted rtl_eff_sem c2 = Some v2 /\ 
-           val_inject (restrict (as_inj mu) (vis mu)) v1 v2.
-Proof.
-  intros.
-  inv SMC; simpl in *; inv HALT.
-  destruct stk; inv H0.
-  destruct stk'.
-  exists v'; split; try reflexivity. eapply VINJ.
-  Print val.
-exists nil.
-  inv MK. split; trivial.
-(*  eapply val_inject_incr; try eassumption.
-    apply restrict_incr.*)
-Qed.*)
+
+
+
+
+
+
+
+
+
+
+
+
+
+
+
+
+
+
+
+
+
+
+
+
+
+
+
+
+
 
 Lemma inject_val_inject_halted: forall (cd : RTL_core) (mu : SM_Injection) (c1 : RTL_core) 
                                        (m1 : mem) (c2 : RTL_core) (m2 : mem) (v1 : val) (MC: MATCH cd mu c1 m1 c2 m2) (Hl: halted rtl_eff_sem c1 = Some v1 ),
@@ -734,17 +897,6 @@ Qed.
 apply MATCH_REACH_REACH.
 
 apply inject_val_inject_halted.
-Lemma at_external_lemma: forall (mu : SM_Injection) (c1 : RTL_core) (m1 : mem) 
-                                (c2 : RTL_core) (m2 : mem) (e : external_function) 
-                                (vals1 : list val) (ef_sig : signature),
-                           MATCH c1 mu c1 m1 c2 m2 ->
-                           at_external rtl_eff_sem c1 = Some (e, ef_sig, vals1) ->
-                           Mem.inject (as_inj mu) m1 m2 /\
-                           (exists vals2 : list val,
-                              Forall2 (val_inject (restrict (as_inj mu) (vis mu))) vals1 vals2 /\
-                              at_external rtl_eff_sem c2 = Some (e, ef_sig, vals2)).
-Admitted.
-apply at_external_lemma.
 
 
 
